examples/RockPaperScissors.lean
@@ -1,0 +1,72 @@
+import Chorlean.Choreo
+import Chorlean.Effects
+import Mathlib.Data.Fintype.Basic
+import Mathlib.Tactic.DeriveFintype
+
+open Effect
+inductive Move   | Rock | Paper | Scissors
+deriving Lean.ToJson, Lean.FromJson, Repr
+
+inductive Result | A | B | Draw
+
+
+instance: ToString Move where toString | .Rock => "Rock" |.Paper => "Paper" |.Scissors => "Scissors"
+
+def wins: Move -> Move -> Bool
+| .Rock, .Scissors | .Scissors, .Paper | .Paper, .Rock => true | _, _ => false
+
+instance: ToString Result where toString | .A => "A" |.B => "B" |.Draw => "Draw"
+
+def eval (a b: Move): Result :=
+  if (wins a b) then
+    .A
+  else if (wins b a) then
+    .B
+  else
+    .Draw
+
+partial def promptMove: IO Move := do
+  IO.println "enter your move (R|P|S)"
+  let line <- IO.getLine
+  match line with
+  | "s" | "S" => return .Scissors
+  | "r" | "R" => return .Rock
+  | "p" | "P" => return .Paper
+  | _ => promptMove
+
+instance: Role where
+  N := 2
+  name | 0 => "A" | 1 => "B"
+
+def A: δ := 0
+def B: δ := 1
+
+variable [Endpoint]
+variable [MonadLiftT NetEff IO]
+
+
+instance: ChorMain where
+  main _ := do
+    let moves <- par promptMove
+    let moves <- gatherAll moves
+    let resAB := eval (moves ⟨A, by decide⟩) (moves ⟨B,by decide⟩)
+
+    let msg: Faceted String := Faceted.of fun id =>
+      match resAB with
+      | .A    => s!"you {if (id = A) then "won" else "lost"}"
+      | .B    => s!"you {if (id = B) then "won" else "lost"}"
+      | .Draw => "Draw!"
+
+    --par $ IO.println (msg rid (by simp; exact RID.is_ep.symm))
+
+    par ( do
+      let myMsg := msg rid
+      let content := myMsg.un (by simp)
+      return ()
+    )
+
+
+    return Faceted.of 0
+
+
+ def main := CHOR_ENTRYPOINT
