README.md
@@ -24,15 +24,16 @@ instance: Role where
 ### Executing Endpoint
 Choreographic code is always executed by a single role that runs those instructions relevant to them.
 This role is an argument for running choreographies, and usually passed by the user when starting the program on the command line.
-Programmers do not have direct access to the endpoint, but only through the libraries API.
-This role is called *ep* for endpoint.
+Programmers do not have direct access to the endpoint, but only through the RID (RoleIDEntity) class.
+The RID class contains a role (RID.id) and evidence that this role is in fact the currently executing one (RID.is_ep).
+*rid* is an abbreviation for RID.id
 
 ### Choreo Monad
 
 Choreographies in ChorLean are written in the *Choreo* Monad.
 *Choreo* is parameterized by:
-- the set of roles that participate in that function (present roles), all other roles will ignore that code. The set is specified as a predicate over roles, where all roles fulfilling that predicate participate 
-- Evidence that the endpoint fulfills the predicate
+- the List of roles that participate in that function (present roles). All other roles will ignore that code. 
+- Evidence that the endpoint is member of this list.
 
 ### Main Entrypoint
 Chorlean provides a function that automatically generates the main function for you, called *CHOR_ENTRYPOINT*, and a main function is expected to be defined as:
@@ -45,14 +46,15 @@ The Main method maps the command line inputs as a faceted list of strings, to a 
 
 ### Located Values and Types
 
-Types in ChorLean are annotated by which roles have knowledge of them by predicates (similar to present roles).
+Types in ChorLean are annotated a list of roles that knowledge of their underlying value.
 They are notated as *α @ p* where *α* is a type and *p* a predicate over roles.
-Located values are defined as functions from evidence, that the endpoint has knowledge of the value (fulfills the predicate), to the value itself. Such evidence can be gathered by *enclaving*.
+Located values are defined as functions from evidence, that the executing role has knowledge of the value (is member of the list), to the value itself. Such evidence can be gathered by *enclaving*.
 Helpful functions around located values include:
 
 - Located.wrap: wraps values into located values
 - Located.flatten: removes one layer of nested located values
-- Located.cast: casts into a located value with different predicate *p'*, if *(p x -> p' x)*. This is also helpful when two propositions describe the same set of roles, like *x ∈ [A]* and *x=A*
+- Located.cast: casts into a located value with different list of owners *p'*, if *p ⊆  p'*. This is helpful when two lists contain the same set of roles but are not equal, like *[A]* and *[A,A]*
+- Located.un: unwraps a located value. Requires an instance of RID and the executing role to be member of the owners. This member proof is tried to be inferred automatically but sometimes has to be entered manually 
 
 #### Faceted
 Maps roles to located values which are located at them. Helpful for parallel computations.
@@ -63,19 +65,19 @@ The Core of ChorLean is built on only 3 functions
 
 1. Enclave: embeds a choreography containing less present roles into a bigger one.
 2. Broadcast: broadcasts a located value to all present roles, such that it can then be used as a non-located value.
-3. Locally: runs a program on the present role. *Requires* a single location to be present.
-
+3. Locally: runs a program on the present role. *Requires* a single location to be present. IO Programs are automatically lifted into the choreography with an RID instance.
 ### Other helpful functions and notations:
 
 #### Enclaves
 
-The examples make use the following notation for enclave: *a ~ b* and *a ° b*, where *a* is something with a membership relation (like lists) and *b* is the subchoreography to enclave. Using the *°*, the result of the enclave is also broadcasted. By *[A]° locally IO.getLine* the Role A would perform a getline program locally and broadcast it afterwards.
+The examples make use the following notation for enclave: *a ~~ b* and *a °° b*, where *a* is a list of roles, being a subset of the currently present ones, and *b* is the subchoreography to enclave. By using the *°°*, the result of the enclave is also broadcasted. By *[A]° IO.getLine* the Role A would perform a getline program locally and broadcast it afterwards.
+There are alternative notations if only a single role is enclaved with only a single symbol *a ~ b* and *a ° b*. These versions provide an RID class instance to the user with access to the currently executing role.
 
 #### Parallel
 
-Iterates over all present roles to perform a program locally on them. The program in this case has knowledge of the identity of the executing role. Results in *faceted* values. A Choreography where every role prints their identity looks like this
+Iterates over all present roles to perform a program locally on them. The program in this case has knowledge of the identity of the executing role by an RID instance. Results in *faceted* values. A Choreography where every role prints their identity might look like this
 ```lean
-par fun id => IO.println s!"hello from {id}"
+par (IO.println s!"hello from {Role.name rid}")
 ```
 
 #### Scatter/Gather
